ReTierProofContext.v
@@ -25,119 +25,271 @@ induction H_transmittable; intros; inversion H_typing.
 Qed.
 
 
+Lemma appears_free_locally_or_remotely : forall t x,
+    appears_free_in_t_locality x t RemoteVar ->
+    appears_free_in_t_locality x t LocalOrRemoteVar.
+Proof.
+intros t x H.
+induction t; simpl; simpl in H.
+- destruct (beq_id x i); try assumption.
+  apply IHt in H.
+  assumption.
+- destruct H.
+  + apply IHt1 in H. left. assumption.
+  + apply IHt2 in H. right. assumption.
+- destruct (beq_id x i); try reflexivity || contradiction.
+- contradiction.
+- contradiction.
+- apply IHt in H. assumption.
+- contradiction.
+- destruct H.
+  + apply IHt1 in H. left. assumption.
+  + apply IHt2 in H. right. assumption.
+- assumption.
+- destruct H.
+  + left. assumption.
+  + apply IHt2 in H. right. assumption.
+- destruct (beq_id x i); destruct H.
+  + apply IHt1 in H. left. assumption.
+  + right. assumption.
+  + apply IHt1 in H. left. assumption.
+  + right. assumption.
+- destruct (beq_id x i); destruct H.
+  + apply IHt1 in H. left. assumption.
+  + destruct H.
+    * right. left. assumption.
+    * apply IHt3 in H. right. right. assumption.
+  + apply IHt1 in H. left. assumption.
+  + destruct H.
+    * right. left. assumption.
+    * apply IHt3 in H. right. right. assumption.
+- apply IHt in H. assumption.
+- apply IHt in H. assumption.
+- apply IHt in H. assumption.
+- destruct H.
+  + apply IHt1 in H. left. assumption.
+  + apply IHt2 in H. right. assumption.
+- contradiction.
+- contradiction.
+- contradiction.
+Qed.
+
+
 Lemma free_in_context_t : forall typing ties Psi Delta Gamma P t T x,
-   appears_free_in_t x t ->
    Context typing ties Psi Delta Gamma P |- t \in T ->
-   exists T', Gamma x = Some T' \/ Delta x = Some (T' on P).
+   (appears_free_in_t_locality x t LocalOrRemoteVar ->
+    exists T' P', Gamma x = Some T' \/ Delta x = Some (T' on P')) /\
+   (appears_free_in_t_locality x t RemoteVar ->
+    exists T' P', Delta x = Some (T' on P')).
 Proof.
 intros until x.
-intros H_free_x H_typing.
+intros H_typing.
 generalize dependent Gamma.
 generalize dependent T.
-induction t; (intros; inversion H_typing; subst).
-- simpl in H_free_x.
-  case_eq (beq_id x i); intros H_eq.
-  + rewrite H_eq in H_free_x.
-    contradiction.
-  + rewrite H_eq in H_free_x.
-    eapply IHt in H_free_x.
-    * { instantiate (1 := (idUpdate i t Gamma)) in H_free_x.
-        inversion H_free_x as [ T' H_lookup ].
-        destruct H_lookup as [ H_lookup | H_lookup ].
-        - exists T'.
-          left.
-          rewrite <- H_lookup.
-          unfold idUpdate, Maps.p_update, Maps.t_update.
-          rewrite H_eq.
-          reflexivity.
-        - exists T'.
-          right.
-          assumption.
-      }
-    * unfold addVarDec in H4.
-      eassumption.
+generalize dependent P.
+induction t; intros; inversion H_typing; subst; split; intros H_free_x; simpl in H_free_x.
+- case_eq (beq_id x i); intros H_eq; rewrite H_eq in H_free_x.
+  + eapply IHt in H_free_x; try eassumption.
+    destruct H_free_x as [ T' H_lookup ], H_lookup as [ P' H_lookup ].
+    exists T', P'.
+    right. assumption.
+  + eapply IHt with (Gamma := (idUpdate i t Gamma)) in H_free_x; try eassumption.
+    destruct
+        H_free_x as [ T' H_lookup ],
+        H_lookup as [ P' H_lookup ],
+        H_lookup as [ H_lookup | H_lookup ].
+    * exists T', P'.
+      left.
+      rewrite <- H_lookup.
+      unfold idUpdate, Maps.p_update, Maps.t_update.
+      rewrite H_eq.
+      reflexivity.
+    * exists T', P'.
+      right. assumption.
+- destruct (beq_id x i).
+  + eapply IHt in H_free_x; eassumption.
+  + eapply IHt in H_free_x; eassumption.
 - destruct H_free_x.
   + eapply IHt1; eassumption.
   + eapply IHt2; eassumption.
-- simpl in H_free_x.
-  case_eq (beq_id x i); intros H_eq.
+- destruct H_free_x.
+  + eapply IHt1; eassumption.
+  + eapply IHt2; eassumption.
+- case_eq (beq_id x i); intros H_eq.
   + rewrite beq_id_eq in H_eq.
     subst.
     unfold getVarEnv, getVarEnv, getPlaceEnv, getPeer in H1.
-    exists T.
+    exists T, P.
     destruct H1.
     * left. assumption.
     * destruct H.
       right; assumption.
   + rewrite H_eq in H_free_x.
     contradiction.
+- destruct (beq_id x i); contradiction.
+- contradiction.
+- contradiction.
 - contradiction.
 - contradiction.
 - eapply IHt; eassumption.
+- eapply IHt; eassumption.
+- contradiction.
 - contradiction.
 - destruct H_free_x.
   + eapply IHt1; eassumption.
   + eapply IHt2; eassumption.
-- eapply IHt; eassumption.
 - destruct H_free_x.
   + eapply IHt1; eassumption.
   + eapply IHt2; eassumption.
 - simpl in H_free_x.
-  case_eq (beq_id x i); intros H_eq.
-  + rewrite H_eq in H_free_x.
-    eapply IHt1; eassumption.
-  + rewrite H_eq in H_free_x.
-    destruct H_free_x as [ H_free_x | H_free_x ].
+  eapply IHt with (Gamma := emptyVarEnv) in H_free_x; try eassumption.
+  destruct
+      H_free_x as [ T' H_lookup ],
+      H_lookup as [ P' H_lookup ],
+      H_lookup as [ H_lookup | H_lookup ].
+  + unfold emptyVarEnv, idEmpty, Maps.p_empty in H_lookup.
+    congruence.
+  + exists T', P'.
+    right. assumption.
+- simpl in H_free_x.
+  eapply IHt with (Gamma := emptyVarEnv) in H_free_x; try eassumption.
+  destruct
+      H_free_x as [ T' H_lookup ],
+      H_lookup as [ P' H_lookup ],
+      H_lookup as [ H_lookup | H_lookup ].
+  + unfold emptyVarEnv, idEmpty, Maps.p_empty in H_lookup.
+    congruence.
+  + exists T', P'.
+    assumption.
+- destruct H_free_x as [ H_free_x | H_free_x ].
+  + eapply IHt1 with (Gamma := emptyVarEnv) in H_free_x; try eassumption.
+    destruct
+        H_free_x as [ T' H_lookup ],
+        H_lookup as [ P' H_lookup ],
+        H_lookup as [ H_lookup | H_lookup ].
+    * unfold emptyVarEnv, idEmpty, Maps.p_empty in H_lookup.
+      congruence.
+    * exists T', P'.
+      right. assumption.
+  + eapply IHt2; eassumption.
+- destruct H_free_x as [ H_free_x | H_free_x ].
+  + eapply IHt1 with (Gamma := emptyVarEnv) in H_free_x; try eassumption.
+    destruct
+        H_free_x as [ T' H_lookup ],
+        H_lookup as [ P' H_lookup ],
+        H_lookup as [ H_lookup | H_lookup ].
+    * unfold emptyVarEnv, idEmpty, Maps.p_empty in H_lookup.
+      congruence.
+    * exists T', P'.
+      assumption.
+  + eapply IHt2; eassumption.
+- case_eq (beq_id x i); intros H_eq; rewrite H_eq in H_free_x.
+  + destruct H_free_x as [ H_free_x | H_free_x ].
     * eapply IHt1; eassumption.
-    * { eapply IHt2 in H_free_x as H_exists_lookup.
-        - instantiate (1 := (idUpdate i T0 Gamma)) in H_exists_lookup.
-          inversion H_exists_lookup as [ T' H_lookup ].
-          destruct H_lookup as [ H_lookup | H_lookup ].
-          + exists T'.
-            left.
-            rewrite <- H_lookup.
-            unfold idUpdate, Maps.p_update, Maps.t_update.
-            rewrite H_eq.
-            reflexivity.
-          + exists T'.
-            right.
-            assumption.
-        - unfold addVarDec in H7.
-          eassumption.
+    * eapply IHt2 with (Gamma := (idUpdate i T0 emptyVarEnv)) in H_free_x; try eassumption.
+      destruct H_free_x as [ T' H_lookup ], H_lookup as [ P' H_lookup ].
+      exists T', P'.
+      right. assumption.
+  + destruct H_free_x as [ H_free_x | H_free_x ].
+    * eapply IHt1; eassumption.
+    * { eapply IHt2 with (Gamma := (idUpdate i T0 emptyVarEnv)) in H_free_x; try eassumption.
+        destruct
+            H_free_x as [ T' H_lookup ],
+            H_lookup as [ P' H_lookup ],
+            H_lookup as [ H_lookup | H_lookup ].
+        - unfold
+            idUpdate, Maps.p_update, Maps.t_update,
+            emptyVarEnv, idEmpty, Maps.p_empty in H_lookup.
+          rewrite H_eq in H_lookup.
+          congruence.
+        - exists T', P'.
+          right. assumption.
       }
-- simpl in H_free_x.
-  case_eq (beq_id x i); intros H_eq.
-  + rewrite H_eq in H_free_x.
-    destruct H_free_x.
+- case_eq (beq_id x i); intros H_eq; rewrite H_eq in H_free_x.
+  + destruct H_free_x.
     * eapply IHt1; eassumption.
-    * eapply IHt3; eassumption.
-  + rewrite H_eq in H_free_x.
-    destruct H_free_x as [ H_free_x | H_free_x ].
+    * eapply IHt2; eassumption.
+  + destruct H_free_x as [ H_free_x | H_free_x ].
+    * eapply IHt1; eassumption.
+    * { eapply IHt2 with (Gamma := (idUpdate i T0 emptyVarEnv)) in H_free_x; try eassumption.
+        destruct
+            H_free_x as [ T' H_lookup ],
+            H_lookup as [ P' H_lookup ],
+            H_lookup as [ H_lookup | H_lookup ].
+        - unfold
+            idUpdate, Maps.p_update, Maps.t_update,
+            emptyVarEnv, idEmpty, Maps.p_empty in H_lookup.
+          rewrite H_eq in H_lookup.
+          congruence.
+        - exists T', P'.
+          assumption.
+      }
+- case_eq (beq_id x i); intros H_eq; rewrite H_eq in H_free_x.
+  * { destruct H_free_x as [ H_free_x | H_free_x ].
+      - eapply IHt1; eassumption.
+      - destruct H_free_x as [ H_free_x | H_free_x ].
+        + eapply IHt2 with (Gamma := (idUpdate i T0 emptyVarEnv)) in H_free_x; try eassumption.
+          destruct H_free_x as [ T' H_lookup ], H_lookup as [ P' H_lookup ].
+          exists T', P'.
+          right. assumption.
+        + eapply IHt3; eassumption.
+    }
+  * { destruct H_free_x as [ H_free_x | H_free_x ].
+      - eapply IHt1; eassumption.
+      - destruct H_free_x as [ H_free_x | H_free_x ].
+        + eapply IHt2 with (Gamma := (idUpdate i T0 emptyVarEnv)) in H_free_x; try eassumption.
+          destruct
+              H_free_x as [ T' H_lookup ],
+              H_lookup as [ P' H_lookup ],
+              H_lookup as [ H_lookup | H_lookup ].
+          * unfold
+              idUpdate, Maps.p_update, Maps.t_update,
+              emptyVarEnv, idEmpty, Maps.p_empty in H_lookup.
+            rewrite H_eq in H_lookup.
+            congruence.
+          * exists T', P'.
+            right. assumption.
+        + eapply IHt3; eassumption.
+    }
+- case_eq (beq_id x i); intros H_eq; rewrite H_eq in H_free_x.
+  + destruct H_free_x as [ H_free_x | H_free_x ].
     * eapply IHt1; eassumption.
     * { destruct H_free_x as [ H_free_x | H_free_x ].
-        - eapply IHt2 in H_free_x as H_exists_lookup.
-          + instantiate (1 := (idUpdate i T0 Gamma)) in H_exists_lookup.
-            inversion H_exists_lookup as [ T' H_lookup ].
-            destruct H_lookup as [ H_lookup | H_lookup ].
-            * exists T'.
-              left.
-              rewrite <- H_lookup.
-              unfold idUpdate, Maps.p_update, Maps.t_update.
-              rewrite H_eq.
-              reflexivity.
-            * exists T'.
-              right.
-              assumption.
-          + unfold addVarDec in H7.
-            eassumption.
+        - eapply IHt2; eassumption.
+        - eapply IHt3; eassumption.
+      }
+  + destruct H_free_x as [ H_free_x | H_free_x ].
+    * eapply IHt1; eassumption.
+    * { destruct H_free_x as [ H_free_x | H_free_x ].
+        - eapply IHt2 with (Gamma := (idUpdate i T0 emptyVarEnv)) in H_free_x; try eassumption.
+          destruct
+              H_free_x as [ T' H_lookup ],
+              H_lookup as [ P' H_lookup ],
+              H_lookup as [ H_lookup | H_lookup ].
+          + unfold
+              idUpdate, Maps.p_update, Maps.t_update,
+              emptyVarEnv, idEmpty, Maps.p_empty in H_lookup.
+            rewrite H_eq in H_lookup.
+            congruence.
+          + exists T', P'.
+            assumption.
         - eapply IHt3; eassumption.
       }
 - eapply IHt; eassumption.
 - eapply IHt; eassumption.
 - eapply IHt; eassumption.
+- eapply IHt; eassumption.
+- eapply IHt; eassumption.
+- eapply IHt; eassumption.
 - destruct H_free_x.
   + eapply IHt1; eassumption.
   + eapply IHt2; eassumption.
+- destruct H_free_x.
+  + eapply IHt1; eassumption.
+  + eapply IHt2; eassumption.
+- contradiction.
+- contradiction.
+- contradiction.
 - contradiction.
 - contradiction.
 - contradiction.
@@ -152,31 +304,33 @@ Proof.
 intros until x.
 intros H_free_x H_typing.
 generalize dependent Delta.
-induction s; (intros; inversion H_typing; subst).
-- simpl in H_free_x.
-  case_eq (beq_id x i); intros H_eq.
-  + rewrite H_eq in H_free_x.
-    eapply free_in_context_t in H5 as H_exists_lookup; try eassumption.
-    destruct H_exists_lookup as [ T' H_lookup ].
-    destruct H_lookup as [ H_lookup | H_lookup ].
+induction s; intros; inversion H_typing; subst; simpl in H_free_x.
+- case_eq (beq_id x i); intros H_eq; rewrite H_eq in H_free_x.
+  + eapply free_in_context_t in H5 as H_lookup; try eassumption.
+    destruct H_lookup as [ H_lookup_Gamma H_lookup_Delta ].
+    destruct H_lookup_Gamma as [ T' H_lookup ]. try eassumption.
+    destruct
+        H_lookup as [ P' H_lookup ],
+        H_lookup as [ H_lookup | H_lookup ].
     * unfold emptyVarEnv, idEmpty, Maps.p_empty in H_lookup.
       congruence.
-    * exists (T' on P).
+    * exists (T' on P').
       assumption.
-  + rewrite H_eq in H_free_x.
-    destruct H_free_x as [ H_free_x | H_free_x ].
-    * { simpl in *.
-        eapply free_in_context_t in H5 as H_exists_lookup; try eassumption.
-        destruct H_exists_lookup as [ T' H_lookup ].
-        destruct H_lookup as [ H_lookup | H_lookup ].
+  + destruct H_free_x as [ H_free_x | H_free_x ].
+    * { eapply free_in_context_t in H5 as H_lookup; try eassumption.
+        destruct H_lookup as [ H_lookup_Gamma H_lookup_Delta ].
+        destruct H_lookup_Gamma as [ T' H_lookup ]. try eassumption.
+        destruct
+            H_lookup as [ P' H_lookup ],
+            H_lookup as [ H_lookup | H_lookup ].
         - unfold emptyVarEnv, idEmpty, Maps.p_empty in H_lookup.
           congruence.
-        - exists (T' on P).
+        - exists (T' on P').
           assumption.
       }
-    * { eapply IHs in H_free_x as H_exists_lookup.
-        - destruct H_exists_lookup as [ T' H_lookup ].
-          exists T'.
+    * { eapply IHs in H_free_x as H_lookup.
+        - destruct H_lookup as [ S' H_lookup ].
+          exists S'.
           instantiate (1 := (idUpdate i (T on P) Delta)) in H_lookup.
           unfold idUpdate, Maps.p_update, Maps.t_update in H_lookup.
           rewrite H_eq in H_lookup.
@@ -189,39 +343,47 @@ Qed.
 
 Lemma context_invariance_t : forall typing ties Psi Delta Delta' Gamma Gamma' P t T,
   Context typing ties Psi Delta Gamma P |- t \in T ->
-  (forall x, appears_free_in_t x t ->
+  (forall x, appears_free_in_t_locality x t LocalOrRemoteVar ->
    Gamma x = Gamma' x /\ (Gamma x = None -> Delta x = Delta' x)) ->
+  (forall x, appears_free_in_t_locality x t RemoteVar ->
+   Delta x = Delta' x) ->
   Context typing ties Psi Delta' Gamma' P |- t \in T.
 Proof.
 intros until T.
-intros H_typing H_free_x.
+intros H_typing H_free_x_Gamma H_free_x_Delta.
 generalize dependent Gamma.
 generalize dependent Gamma'.
 generalize dependent T.
-induction t; intros; (intros; inversion H_typing).
+generalize dependent P.
+induction t; intros; inversion H_typing.
 - eapply IHt in H4.
   + apply T_Abs. simpl. eassumption.
-  + intros.
-    subst.
+  + intros y H_free_y.
+    apply H_free_x_Delta.
+    simpl.
+    destruct (beq_id y i); assumption.
+  + intros y H_free_y.
     unfold idUpdate, Maps.p_update, Maps.t_update.
-    case_eq (beq_id x0 i); intros H_eq.
+    case_eq (beq_id y i); intros H_eq.
     * split; congruence.
-    * apply H_free_x.
+    * apply H_free_x_Gamma.
       simpl.
       rewrite H_eq.
       assumption.
 - eapply IHt1 in H2.
   + eapply IHt2 in H4.
     * eapply T_App; eassumption.
-    * intros. apply H_free_x. simpl. right. assumption.
-  + intros. apply H_free_x. simpl. left. assumption.
+    * intros. apply H_free_x_Delta. simpl. right. assumption.
+    * intros. apply H_free_x_Gamma. simpl. right. assumption.
+  + intros. apply H_free_x_Delta. simpl. left. assumption.
+  + intros. apply H_free_x_Gamma. simpl. left. assumption.
 - simpl in H1.
   apply T_Var.
   simpl.
-  specialize H_free_x with i.
-  simpl in H_free_x.
-  rewrite beq_id_refl in H_free_x.
-  destruct H_free_x as [ H_Gamma H_Gamma_Delta ]; try reflexivity.
+  specialize H_free_x_Gamma with i.
+  simpl in H_free_x_Gamma.
+  rewrite beq_id_refl in H_free_x_Gamma.
+  destruct H_free_x_Gamma as [ H_Gamma H_Gamma_Delta ]; try reflexivity.
   rewrite <- H_Gamma.
   destruct H1 as [ H_lookup_Gamma | H_lookup_Delta ].
   + left. assumption.
@@ -233,81 +395,131 @@ induction t; intros; (intros; inversion H_typing).
 - apply T_None.
 - eapply IHt in H1.
   + eapply T_Some; eassumption.
-  + intros. apply H_free_x. assumption.
+  + intros. apply H_free_x_Delta. assumption.
+  + intros. apply H_free_x_Gamma. assumption.
 - apply T_Nil.
 - eapply IHt1 in H2.
   + eapply IHt2 in H4.
     * eapply T_Cons; eassumption.
-    * intros. apply H_free_x. right. assumption.
-  + intros. apply H_free_x. left. assumption.
-- eapply IHt in H2.
+    * intros. apply H_free_x_Delta. simpl. right. assumption.
+    * intros. apply H_free_x_Gamma. simpl. right. assumption.
+  + intros. apply H_free_x_Delta. simpl. left. assumption.
+  + intros. apply H_free_x_Gamma. simpl. left. assumption.
+- eapply IHt in H3.
   + eapply T_AsLocal; eassumption.
-  + intros. apply H_free_x. assumption.
-- eapply IHt1 in H4.
-  + eapply IHt2 in H7.
-    * eapply T_AsLocalFrom; eassumption.
-    * intros. apply H_free_x. right. assumption.
-  + intros. apply H_free_x. left. assumption.
+  + intros.
+    apply H_free_x_Delta.
+    simpl.
+    apply appears_free_locally_or_remotely in H8.
+    assumption.
+  + intros.
+    split; try reflexivity.
+    intros.
+    apply H_free_x_Delta. simpl. assumption.
 - eapply IHt1 in H5.
-  + eapply IHt2 in H7.
+  + eapply IHt2 in H8.
+    * eapply T_AsLocalFrom; eassumption.
+    * intros. apply H_free_x_Delta. simpl. right. assumption.
+    * intros. apply H_free_x_Gamma. simpl. right. assumption.
+  + intros.
+    apply H_free_x_Delta.
+    simpl.
+    left.
+    apply appears_free_locally_or_remotely in H9.
+    assumption.
+  + intros.
+    split; try reflexivity.
+    intros.
+    apply H_free_x_Delta. simpl. left. assumption.
+- eapply IHt1 in H6.
+  + eapply IHt2 in H8.
     * eapply T_Comp; eassumption.
-    * { intros.
-        subst.
-        unfold idUpdate, Maps.p_update, Maps.t_update.
-        case_eq (beq_id x0 i); intros H_eq.
-        - split; reflexivity || congruence.
-        - apply H_free_x.
-          simpl.
-          rewrite H_eq.
+    * { intros y H_free_y.
+        apply H_free_x_Delta.
+        simpl.
+        destruct (beq_id y i).
+        - right. assumption.
+        - apply appears_free_locally_or_remotely in H_free_y.
           right. assumption.
       }
-  + intros.
-    apply H_free_x.
-    simpl.
-    case (beq_id x0 i); try assumption.
-    left. assumption.
-- eapply IHt1 in H7.
-  + eapply IHt2 in H8.
-    * { eapply IHt3 in H10.
-        - eapply T_ComFrom; eassumption.
-        - intros.
-          apply H_free_x.
-          simpl.
-          case (beq_id x0 i).
-          + right. assumption.
-          + right. right. assumption.
+    * { intros y H_free_y.
+        split; try reflexivity.
+        intros H_empty.
+        apply H_free_x_Delta.
+        simpl.
+        unfold idUpdate, Maps.p_update, Maps.t_update in H_empty.
+        destruct (beq_id y i).
+        - congruence.
+        - right. assumption.
       }
-    * { intros.
-        unfold idUpdate, Maps.p_update, Maps.t_update.
-        case_eq (beq_id x0 i); intros H_eq.
-        - split; reflexivity || congruence.
-        - apply H_free_x.
+  + intros y H_free_y.
+    apply H_free_x_Delta.
+    simpl.
+    destruct (beq_id y i); left; assumption.
+  + intros y H_free_y.
+    apply H_free_x_Gamma.
+    simpl.
+    destruct (beq_id y i); left; assumption.
+- eapply IHt1 in H8.
+  + eapply IHt2 in H9.
+    * { eapply IHt3 in H11.
+        - eapply T_ComFrom; eassumption.
+        - intros y H_free_y.
+          apply H_free_x_Delta.
           simpl.
-          rewrite H_eq.
+          destruct (beq_id y i); right; right; assumption.
+        - intros y H_free_y.
+          apply H_free_x_Gamma.
+          simpl.
+          destruct (beq_id y i); right; right; assumption.
+      }
+    * { intros y H_free_y.
+        apply H_free_x_Delta.
+        simpl.
+        destruct (beq_id y i).
+        - right. left. assumption.
+        - apply appears_free_locally_or_remotely in H_free_y.
           right. left. assumption.
       }
-  + intros.
-    apply H_free_x.
+    * { intros y H_free_y.
+        split; try reflexivity.
+        intros H_empty.
+        apply H_free_x_Delta.
+        simpl.
+        unfold idUpdate, Maps.p_update, Maps.t_update in H_empty.
+        destruct (beq_id y i).
+        - congruence.
+        - right. left. assumption.
+      }
+  + intros y H_free_y.
+    apply H_free_x_Delta.
     simpl.
-    case (beq_id x0 i); left; assumption.
+    destruct (beq_id y i); left; assumption.
+  + intros y H_free_y.
+    apply H_free_x_Gamma.
+    simpl.
+    destruct (beq_id y i); left; assumption.
 - eapply IHt in H1.
   + eapply T_Signal; eassumption.
-  + intros. apply H_free_x. assumption.
+  + intros. apply H_free_x_Delta. assumption.
+  + intros. apply H_free_x_Gamma. assumption.
 - eapply IHt in H1.
   + eapply T_ReactiveVar; eassumption.
-  + intros. apply H_free_x. assumption.
+  + intros. apply H_free_x_Delta. assumption.
+  + intros. apply H_free_x_Gamma. assumption.
 - eapply IHt in H0.
   + eapply T_Now; eassumption.
-  + intros. apply H_free_x. assumption.
+  + intros. apply H_free_x_Delta. assumption.
+  + intros. apply H_free_x_Gamma. assumption.
 - eapply IHt1 in H2.
   + eapply IHt2 in H4.
     * eapply T_Set; eassumption.
-    * intros. apply H_free_x. right. assumption.
-  + intros. apply H_free_x. left. assumption.
-- apply T_Peer.
-  assumption.
-- apply T_Reactive.
-  assumption.
+    * intros. apply H_free_x_Delta. simpl. right. assumption.
+    * intros. apply H_free_x_Gamma. simpl. right. assumption.
+  + intros. apply H_free_x_Delta. simpl. left. assumption.
+  + intros. apply H_free_x_Gamma. simpl. left. assumption.
+- apply T_Peer; assumption.
+- apply T_Reactive; assumption.
 - apply T_Nat.
 Qed.
 
@@ -325,14 +537,18 @@ induction s; (intros; inversion H_typing; subst).
 - eapply IHs in H2.
   + eapply T_Place; try eassumption.
     simpl.
-    eapply context_invariance_t; try eassumption.
-    split; try reflexivity.
-    unfold emptyVarEnv, idEmpty, Maps.p_empty.
-    intros.
-    apply H_free_x.
-    simpl.
-    case (beq_id x i); try assumption.
-    left. assumption.
+    eapply context_invariance_t; try eassumption; intros.
+    * split; try reflexivity.
+      intros.
+      apply H_free_x.
+      simpl.
+      case (beq_id x i); try assumption.
+      left. assumption.
+    * apply H_free_x.
+      simpl.
+      apply appears_free_locally_or_remotely in H.
+      case (beq_id x i); try assumption.
+      left. assumption.
   + intros.
     unfold idUpdate, Maps.p_update, Maps.t_update.
     case_eq (beq_id x i); intros H_eq; try reflexivity.
@@ -353,8 +569,8 @@ intros until T.
 intros H_typing x H_free_x.
 eapply free_in_context_t in H_free_x; try eassumption.
 unfold emptyVarEnv, emptyPlaceEnv, idEmpty, Maps.p_empty in H_free_x.
-inversion H_free_x.
-destruct H; congruence.
+destruct H_free_x as [ T' H_lookup ], H_lookup as [ P' H_lookup ].
+destruct H_lookup; congruence.
 Qed.
 
 
